packet number

src/QUIC.Spec.Base.fst
@@ -1,19 +1,12 @@
 module QUIC.Spec.Base
 
 module FB = FStar.Bytes
+module U62 = QUIC.UInt62
 module U64 = FStar.UInt64
 module U32 = FStar.UInt32
 module U8 = FStar.UInt8
 module S = FStar.Seq
-
-inline_for_extraction
-let uint62_bound : (uint62_bound: U64.t { U64.v uint62_bound == pow2 62 }) =
-  [@inline_let] let v = 4611686018427387904uL in
-  [@inline_let] let _ = assert_norm (U64.v v == pow2 62) in
-  v
-
-inline_for_extraction
-let uint62_t = (x: U64.t { U64.v x < U64.v uint62_bound })
+module PN = QUIC.Spec.PacketNumber
 
 type byte = FStar.UInt8.t
 type bytes = s:S.seq byte
@@ -29,36 +22,30 @@ let token_max_len = 16383 // arbitrary bound
 
 inline_for_extraction
 noextract
-type packet_number_length_t : eqtype = (x: U32.t { 1 <= U32.v x /\ U32.v x <= 4 })
-
-inline_for_extraction
-noextract
 let bitfield
   (sz: nat { sz <= 8 })
 : Tot eqtype
 = (x: U8.t { U8.v x < pow2 sz })
 
-(* NOTE: in the following header type, payload_length contains the
-length of the actual payload, NOT including the length of the packet
-number. *)
+type payload_and_pn_length_t = (payload_and_pn_length: U62.t { U64.v payload_and_pn_length >= 20 })
 
 noeq
 type long_header_specifics =
 | MInitial:
   (token: vlbytes 0 token_max_len) -> // arbitrary bound
-  (payload_length: uint62_t) ->
-  (packet_number_length: packet_number_length_t { U64.v payload_length + U32.v packet_number_length < pow2 62 }) ->
-  (packet_number: uint62_t) ->
+  (payload_and_pn_length: payload_and_pn_length_t) ->
+  (packet_number_length: PN.packet_number_length_t) ->
+  (packet_number: PN.packet_number_t) ->
   long_header_specifics
 | MZeroRTT:
-  (payload_length: uint62_t) ->
-  (packet_number_length: packet_number_length_t { U64.v payload_length + U32.v packet_number_length < pow2 62 }) ->
-  (packet_number: uint62_t) ->
+  (payload_and_pn_length: payload_and_pn_length_t) ->
+  (packet_number_length: PN.packet_number_length_t) ->
+  (packet_number: PN.packet_number_t) ->
   long_header_specifics
 | MHandshake:
-  (payload_length: uint62_t) ->
-  (packet_number_length: packet_number_length_t { U64.v payload_length + U32.v packet_number_length < pow2 62 }) ->
-  (packet_number: uint62_t) ->
+  (payload_and_pn_length: payload_and_pn_length_t) ->
+  (packet_number_length: PN.packet_number_length_t) ->
+  (packet_number: PN.packet_number_t) ->
   long_header_specifics
 | MRetry:
   (unused: bitfield 4) ->
@@ -77,8 +64,8 @@ type header =
   (spin: bool) ->
   (key_phase: bool) ->
   (dcid: vlbytes 0 20) ->
-  (packet_number_length: packet_number_length_t) ->
-  (packet_number: uint62_t) ->
+  (packet_number_length: PN.packet_number_length_t) ->
+  (packet_number: PN.packet_number_t) ->
   header
 
 let is_initial (h: header) : Tot bool =
@@ -93,7 +80,7 @@ let is_handshake (h: header) : Tot bool =
 let is_retry (h: header) : Tot bool =
   if MLong? h then MRetry? (MLong?.spec h) else false
 
-let pn_length (h: header { ~ (is_retry h) }) : Tot packet_number_length_t =
+let pn_length (h: header { ~ (is_retry h) }) : Tot PN.packet_number_length_t =
   match h with
   | MLong _ _ _ spec ->
     begin match spec with
@@ -103,7 +90,7 @@ let pn_length (h: header { ~ (is_retry h) }) : Tot packet_number_length_t =
     end
   | MShort _ _ _ pnl _ -> pnl
 
-let packet_number (h: header {~ (is_retry h)}) : Tot uint62_t =
+let packet_number (h: header {~ (is_retry h)}) : Tot PN.packet_number_t =
   match h with
   | MLong _ _ _ spec ->
     begin match spec with
@@ -120,27 +107,6 @@ let dcid_len (h: header) : Tot nat =
 
 type packet = b:bytes{let l = S.length b in (* 21 <= l /\ *) l < pow2 32}
 
-(* Packet number *)
-
-inline_for_extraction
-let last_packet_number_t = (last: uint62_t { U64.v last + 1 < U64.v uint62_bound})
-
-let bound_npn' (pn_len:nat { pn_len < 4 }) : Tot (y: nat {y == pow2 (8 `op_Multiply` (pn_len + 1)) }) =
-  assert_norm (pow2 8 == 256);
-  assert_norm (pow2 16 == 65536);
-  assert_norm (pow2 24 == 16777216);
-  assert_norm (pow2 32 == 4294967296);
-  match pn_len with
-  | 0 -> 256
-  | 1 -> 65536
-  | 2 -> 16777216
-  | 3 -> 4294967296
-
-let in_window (pn_len: nat { pn_len < 4 }) (last pn:nat) =
-  let h = bound_npn' pn_len in
-  (last+1 < h/2 /\ pn < h) \/
-  (last+1 >= U64.v uint62_bound - h/2 /\ pn >= U64.v uint62_bound - h) \/
-  (last+1 - h/2 < pn /\ pn <= last+1 + h/2)
 
 (* Payload length *)
 
@@ -151,7 +117,7 @@ let has_payload_length
 
 let payload_length 
   (h: header { has_payload_length h })
-: Tot uint62_t
+: Tot U62.t
 = match MLong?.spec h with
   | MInitial _ pl _ _ -> pl
   | MZeroRTT pl _ _ -> pl
@@ -159,6 +125,8 @@ let payload_length
 
 (* Correctness of a packet wrt. parsing parameters (cid_len, window) *)
 
+module Secret = Lib.IntTypes
+
 let is_valid_header (h: header) (cid_len: nat) (last: nat) : Tot Type0 =
   (MShort? h ==> dcid_len h == cid_len) /\
-  ((~ (is_retry h)) ==> in_window (U32.v (pn_length h) - 1) last (U64.v (packet_number h)))
+  ((~ (is_retry h)) ==> PN.in_window (Secret.v (pn_length h) - 1) last (Secret.v (packet_number h)))
