src/QUIC.Spec.PacketNumber.fsti
@@ -1,27 +1,57 @@
 module QUIC.Spec.PacketNumber
-open QUIC.Spec.Base
 open LowParse.Spec.Base
 
+module U62 = QUIC.UInt62
 module U64 = FStar.UInt64
 module U32 = FStar.UInt32
+module Secret = Lib.IntTypes
+
+inline_for_extraction
+noextract
+type packet_number_length_t = (x: Secret.uint32 { 1 <= Secret.v x /\ Secret.v x <= 4 })
 
 inline_for_extraction
 let parse_packet_number_kind
   (sz: packet_number_length_t)
 : Tot parser_kind
-= total_constant_size_parser_kind (U32.v sz)
+= total_constant_size_parser_kind (Secret.v sz)
+
+(* Packet number *)
 
 inline_for_extraction
-let packet_number_t
+let last_packet_number_t = (last: U62.secret { Secret.v last + 1 < U62.v U62.bound})
+
+let bound_npn' (pn_len:nat { pn_len < 4 }) : Tot (y: nat {y == pow2 (8 `op_Multiply` (pn_len + 1)) }) =
+  assert_norm (pow2 8 == 256);
+  assert_norm (pow2 16 == 65536);
+  assert_norm (pow2 24 == 16777216);
+  assert_norm (pow2 32 == 4294967296);
+  match pn_len with
+  | 0 -> 256
+  | 1 -> 65536
+  | 2 -> 16777216
+  | 3 -> 4294967296
+
+let in_window (pn_len: nat { pn_len < 4 }) (last pn:nat) =
+  let h = bound_npn' pn_len in
+  (last+1 < h/2 /\ pn < h) \/
+  (last+1 >= U62.v U62.bound - h/2 /\ pn >= U62.v U62.bound - h) \/
+  (last+1 - h/2 < pn /\ pn <= last+1 + h/2)
+
+inline_for_extraction
+let packet_number_t = U62.secret
+
+inline_for_extraction
+let packet_number_t'
   (last: last_packet_number_t)
   (pn_len: packet_number_length_t)
-: Tot eqtype
-= (pn: uint62_t { in_window (U32.v pn_len - 1) (U64.v last) (U64.v pn) })
+: Tot Type0
+= (pn: packet_number_t { in_window (Secret.v pn_len - 1) (Secret.v last) (Secret.v pn) })
 
 val parse_packet_number
   (last: last_packet_number_t)
   (pn_len: packet_number_length_t)
-: Tot (parser (parse_packet_number_kind pn_len) (packet_number_t last pn_len))
+: Tot (parser (parse_packet_number_kind pn_len) (packet_number_t' last pn_len))
 
 val serialize_packet_number
   (last: last_packet_number_t)
@@ -31,11 +61,11 @@ val serialize_packet_number
 val serialize_packet_number_ext
   (last1 last2: last_packet_number_t)
   (pn_len: packet_number_length_t)
-  (pn: uint62_t)
+  (pn: packet_number_t)
 : Lemma
   (requires (
-    in_window (U32.v pn_len - 1) (U64.v last1) (U64.v pn) /\
-    in_window (U32.v pn_len - 1) (U64.v last2) (U64.v pn)
+    in_window (Secret.v pn_len - 1) (Secret.v last1) (Secret.v pn) /\
+    in_window (Secret.v pn_len - 1) (Secret.v last2) (Secret.v pn)
   ))
   (ensures (
     serialize (serialize_packet_number last1 pn_len) pn == serialize (serialize_packet_number last2 pn_len) pn
