src/QUIC.Secret.fst
@@ -1,0 +1,395 @@
+module QUIC.Secret
+include Lib.IntTypes
+
+module U8 = FStar.UInt8
+module U16 = FStar.UInt16
+module U32 = FStar.UInt32
+module U64 = FStar.UInt64
+
+noextract
+noeq
+type must_inline =
+
+noextract
+unfold
+let norm = norm [delta_attr [(`%must_inline)]; iota; zeta; primops]
+
+noextract
+let supported_type = function
+  | U8 | U16 | U32 | U64 -> true
+  | _ -> false
+
+(* Logic *)
+
+inline_for_extraction
+noextract
+[@"opaque_to_smt"]
+let logand_one_bit
+  (#t: inttype { supported_type t })
+  (#sec: secrecy_level)
+  (x: int_t t sec { v x == 0 \/ v x == 1 })
+  (y: int_t t sec { v y == 0 \/ v y == 1 })
+: Tot (z: int_t t sec { v z == (if v x = 1 && v y = 1 then 1 else 0) })
+= x `mul` y
+
+let logor_one_bit_8
+  (sec: secrecy_level)
+  (x: int_t U8 sec { v x == 0 \/ v x == 1 })
+  (y: int_t U8 sec { v y == 0 \/ v y == 1 })
+: Lemma
+  (v (x `logor` y) == (if v x = 1 || v y = 1 then 1 else 0))
+= logor_spec x y;
+  allow_inversion secrecy_level;
+  assert (U8.logor 0uy 0uy == 0uy);
+  assert (U8.logor 0uy 1uy == 1uy);
+  assert (U8.logor 1uy 0uy == 1uy);
+  assert (U8.logor 1uy 1uy == 1uy)
+
+let logor_one_bit_16
+  (sec: secrecy_level)
+  (x: int_t U16 sec { v x == 0 \/ v x == 1 })
+  (y: int_t U16 sec { v y == 0 \/ v y == 1 })
+: Lemma
+  (v (x `logor` y) == (if v x = 1 || v y = 1 then 1 else 0))
+= logor_spec x y;
+  allow_inversion secrecy_level;
+  assert (U16.logor 0us 0us == 0us);
+  assert (U16.logor 0us 1us == 1us);
+  assert (U16.logor 1us 0us == 1us);
+  assert (U16.logor 1us 1us == 1us)
+
+let logor_one_bit_32
+  (sec: secrecy_level)
+  (x: int_t U32 sec { v x == 0 \/ v x == 1 })
+  (y: int_t U32 sec { v y == 0 \/ v y == 1 })
+: Lemma
+  (v (x `logor` y) == (if v x = 1 || v y = 1 then 1 else 0))
+= logor_spec x y;
+  allow_inversion secrecy_level;
+  assert (U32.logor 0ul 0ul == 0ul);
+  assert (U32.logor 0ul 1ul == 1ul);
+  assert (U32.logor 1ul 0ul == 1ul);
+  assert (U32.logor 1ul 1ul == 1ul)
+
+let logor_one_bit_64
+  (sec: secrecy_level)
+  (x: int_t U64 sec { v x == 0 \/ v x == 1 })
+  (y: int_t U64 sec { v y == 0 \/ v y == 1 })
+: Lemma
+  (v (x `logor` y) == (if v x = 1 || v y = 1 then 1 else 0))
+= logor_spec x y;
+  allow_inversion secrecy_level;
+  assert (U64.logor 0uL 0uL == 0uL);
+  assert (U64.logor 0uL 1uL == 1uL);
+  assert (U64.logor 1uL 0uL == 1uL);
+  assert (U64.logor 1uL 1uL == 1uL)
+
+let logor_one_bit'
+  (#t: inttype { supported_type t })
+  (#sec: secrecy_level)
+  (x: int_t t sec { v x == 0 \/ v x == 1 })
+  (y: int_t t sec { v y == 0 \/ v y == 1 })
+: Lemma
+  (v (x `logor` y) == (if v x = 1 || v y = 1 then 1 else 0))
+= match t with
+  | U8 -> logor_one_bit_8 sec x y
+  | U16 -> logor_one_bit_16 sec x y
+  | U32 -> logor_one_bit_32 sec x y
+  | U64 -> logor_one_bit_64 sec x y
+
+inline_for_extraction
+[@"opaque_to_smt"]
+noextract
+let logor_one_bit
+  (#t: inttype { supported_type t })
+  (#sec: secrecy_level)
+  (x: int_t t sec { v x == 0 \/ v x == 1 })
+  (y: int_t t sec { v y == 0 \/ v y == 1 })
+: Tot (z: int_t t sec { v z == (if v x = 1 || v y = 1 then 1 else 0) })
+= logor_one_bit' x y;
+  x `logor` y
+
+let logxor_one_bit_8
+  (sec: secrecy_level)
+  (x: int_t U8 sec { v x == 0 \/ v x == 1 })
+  (y: int_t U8 sec { v y == 0 \/ v y == 1 })
+: Lemma
+  (v (x `logxor` y) == (if v x = v y then 0 else 1))
+= logxor_spec x y;
+  allow_inversion secrecy_level;
+  assert (U8.logxor 0uy 0uy == 0uy);
+  assert (U8.logxor 0uy 1uy == 1uy);
+  assert (U8.logxor 1uy 0uy == 1uy);
+  assert (U8.logxor 1uy 1uy == 0uy)
+
+let logxor_one_bit_16
+  (sec: secrecy_level)
+  (x: int_t U16 sec { v x == 0 \/ v x == 1 })
+  (y: int_t U16 sec { v y == 0 \/ v y == 1 })
+: Lemma
+  (v (x `logxor` y) == (if v x = v y then 0 else 1))
+= logxor_spec x y;
+  allow_inversion secrecy_level;
+  assert (U16.logxor 0us 0us == 0us);
+  assert (U16.logxor 0us 1us == 1us);
+  assert (U16.logxor 1us 0us == 1us);
+  assert (U16.logxor 1us 1us == 0us)
+
+let logxor_one_bit_32
+  (sec: secrecy_level)
+  (x: int_t U32 sec { v x == 0 \/ v x == 1 })
+  (y: int_t U32 sec { v y == 0 \/ v y == 1 })
+: Lemma
+  (v (x `logxor` y) == (if v x = v y then 0 else 1))
+= logxor_spec x y;
+  allow_inversion secrecy_level;
+  assert (U32.logxor 0ul 0ul == 0ul);
+  assert (U32.logxor 0ul 1ul == 1ul);
+  assert (U32.logxor 1ul 0ul == 1ul);
+  assert (U32.logxor 1ul 1ul == 0ul)
+
+let logxor_one_bit_64
+  (sec: secrecy_level)
+  (x: int_t U64 sec { v x == 0 \/ v x == 1 })
+  (y: int_t U64 sec { v y == 0 \/ v y == 1 })
+: Lemma
+  (v (x `logxor` y) == (if v x = v y then 0 else 1))
+= logxor_spec x y;
+  allow_inversion secrecy_level;
+  assert (U64.logxor 0uL 0uL == 0uL);
+  assert (U64.logxor 0uL 1uL == 1uL);
+  assert (U64.logxor 1uL 0uL == 1uL);
+  assert (U64.logxor 1uL 1uL == 0uL)
+
+let logxor_one_bit'
+  (#t: inttype { supported_type t })
+  (#sec: secrecy_level)
+  (x: int_t t sec { v x == 0 \/ v x == 1 })
+  (y: int_t t sec { v y == 0 \/ v y == 1 })
+: Lemma
+  (v (x `logxor` y) == (if v x = v y then 0 else 1))
+= match t with
+  | U8 -> logxor_one_bit_8 sec x y
+  | U16 -> logxor_one_bit_16 sec x y
+  | U32 -> logxor_one_bit_32 sec x y
+  | U64 -> logxor_one_bit_64 sec x y
+
+inline_for_extraction
+noextract
+[@"opaque_to_smt"]
+let logxor_one_bit
+  (#t: inttype { supported_type t })
+  (#sec: secrecy_level)
+  (x: int_t t sec { v x == 0 \/ v x == 1 })
+  (y: int_t t sec { v y == 0 \/ v y == 1 })
+: Tot (z: int_t t sec { v z == (if v x = v y then 0 else 1) })
+= logxor_one_bit' x y;
+  x `logxor` y
+
+inline_for_extraction
+noextract
+[@"opaque_to_smt"]
+let secret_bool
+  (#t: inttype { supported_type t })
+  (#sec: secrecy_level)
+  (x: bool)
+: Tot (z: int_t t sec { v z == (if x then 1 else 0) })
+= Secret.cast t sec (if x then 1uy else 0uy)
+
+inline_for_extraction
+noextract
+[@"opaque_to_smt"]
+let lognot_one_bit
+  (#t: inttype { supported_type t })
+  (#sec: secrecy_level)
+  (x: int_t t sec { v x == 0 \/ v x == 1 })
+: Tot (z: int_t t sec { v z == (if v x = 1 then 0 else 1) })
+= x `logxor_one_bit` secret_bool true
+
+(* Decomposition *)
+
+module U = FStar.UInt
+
+#push-options "--z3rlimit 16"
+
+inline_for_extraction
+noextract
+[@"opaque_to_smt"]
+let rem2
+  (#t: inttype { supported_type t })
+  (#sec: secrecy_level)
+  (x: int_t t sec)
+: Tot (z: int_t t sec { v z == v x % 2 })
+= 
+  Secret.logand_spec x (Secret.cast t sec 1uy);
+  assert_norm (pow2 1 == 2);
+  U.logand_mask #(bits t) (Secret.v x) 1;
+  x `logand` Secret.cast t sec 1uy
+
+inline_for_extraction
+noextract
+[@"opaque_to_smt"]
+let div2
+  (#t: inttype { supported_type t })
+  (#sec: secrecy_level)
+  (x: int_t t sec)
+: Tot (z: int_t t sec { v z == v x / 2 })
+= x `Secret.shift_right` 1ul
+
+(* Comparisons *)
+
+[@must_inline "opaque_to_smt"]
+noextract
+let rec secret_is_nonzero
+  (#t: inttype { supported_type t })
+  (#sec: secrecy_level)
+  (size: nat)
+  (x: int_t t sec { Secret.v x < pow2 size })
+: Tot (y: int_t t sec {
+    v y == (if v x = 0 then 0 else 1)
+  })
+  (decreases size)
+= if size = 0
+  then secret_bool false
+  else
+    let test_mod = rem2 x in
+    let re = secret_is_nonzero (size - 1) (div2 x) in
+    test_mod `logor_one_bit` re
+
+noextract
+[@must_inline "opaque_to_smt"]
+let rec secrets_are_different
+  (#t: inttype { supported_type t })
+  (#sec: secrecy_level)
+  (size: nat)
+  (x: int_t t sec { Secret.v x < pow2 size })
+  (y: int_t t sec { Secret.v y < pow2 size })
+: Tot (z: int_t t sec {
+    v z == (if v x <> v y then 1 else 0)
+  })
+  (decreases size)
+= 
+  if size = 0
+  then secret_bool false
+  else
+    let xm = rem2 x in
+    let ym = rem2 y in
+    let test_mod = xm `logxor_one_bit` ym in
+    let re = secrets_are_different (size - 1) (div2 x) (div2 y) in
+    test_mod `logor_one_bit` re
+
+noextract
+[@must_inline "opaque_to_smt"]
+let secrets_are_equal
+  (#t: inttype { supported_type t })
+  (#sec: secrecy_level)
+  (size: nat)
+  (x: int_t t sec { Secret.v x < pow2 size })
+  (y: int_t t sec { Secret.v y < pow2 size })
+: Tot (z: int_t t sec {
+    v z == (if v x = v y then 1 else 0)
+  })
+= lognot_one_bit (secrets_are_different size x y)
+
+inline_for_extraction
+noextract
+[@"opaque_to_smt"]
+let one_bit_lt
+  (#t: inttype { supported_type t })
+  (#sec: secrecy_level)
+  (x: int_t t sec { v x == 0 \/ v x == 1 })
+  (y: int_t t sec { v y == 0 \/ v y == 1 })
+: Tot (z: int_t t sec { v z == (if v x < v y then 1 else 0) })
+= lognot_one_bit x `logand_one_bit` y
+
+inline_for_extraction
+noextract
+[@"opaque_to_smt"]
+let one_bit_eq
+  (#t: inttype { supported_type t })
+  (#sec: secrecy_level)
+  (x: int_t t sec { v x == 0 \/ v x == 1 })
+  (y: int_t t sec { v y == 0 \/ v y == 1 })
+: Tot (z: int_t t sec { v z == (if v x = v y then 1 else 0) })
+= lognot_one_bit (x `logxor_one_bit` y)
+
+(* This works, but is very slow.
+noextract
+[@must_inline]
+let rec secret_is_lt
+  (#t: inttype { supported_type t })
+  (#sec: secrecy_level)
+  (size: nat)
+  (x: int_t t sec { v x < pow2 size })
+  (y: int_t t sec { v y < pow2 size })
+: Tot (z: int_t t sec { v z == (if v x < v y then 1 else 0) })
+  (decreases size)
+= if size = 0
+  then secret_bool false
+  else
+    secret_is_lt (size - 1) (div2 x) (div2 y) `logor_one_bit`
+    (secrets_are_equal (size - 1) (div2 x) (div2 y) `logand_one_bit` one_bit_lt (rem2 x) (rem2 y)) 
+*)
+
+inline_for_extraction
+noextract
+[@"opaque_to_smt"]
+let highest_bit
+  (#t: inttype { supported_type t })
+  (#sec: secrecy_level)
+  (size: nat { size > 0 /\ size <= bits t })
+  (x: int_t t sec { v x < pow2 (size) })
+: Tot (z: int_t t sec { v z == v x / pow2 (size - 1) /\ (v z == 0 \/ v z == 1) })
+= x `shift_right` Secret.mk_int (size - 1)
+
+inline_for_extraction
+noextract
+[@"opaque_to_smt"]
+let lowest_bits
+  (#t: inttype { supported_type t })
+  (#sec: secrecy_level)
+  (size: nat { size > 0 /\ size <= bits t })
+  (x: int_t t sec { v x < pow2 (size) })
+: Tot (z: int_t t sec { v z == v x % pow2 (size - 1) })
+= FStar.Math.Lemmas.pow2_le_compat (bits t) (size); 
+  x `logand` mod_mask (Secret.mk_int (size - 1))
+
+noextract
+[@must_inline "opaque_to_smt"]
+let rec secret_is_lt
+  (#t: inttype { supported_type t })
+  (#sec: secrecy_level)
+  (size: nat { size <= bits t })
+  (x: int_t t sec { v x < pow2 (size) })
+  (y: int_t t sec { v y < pow2 (size) })
+: Tot (z: int_t t sec { v z == (if v x < v y then 1 else 0) })
+  (decreases (size))
+= if size = 0
+  then secret_bool false
+  else
+    let xh = highest_bit size x in
+    let xl = lowest_bits size x in
+    let yh = highest_bit size y in
+    let yl = lowest_bits size y in
+    (xh `one_bit_lt` yh) `logor_one_bit`
+    ((xh `one_bit_eq` yh) `logand_one_bit` secret_is_lt (size - 1) xl yl)
+
+noextract
+[@must_inline "opaque_to_smt"]
+let rec secret_is_le
+  (#t: inttype { supported_type t })
+  (#sec: secrecy_level)
+  (size: nat { size <= bits t })
+  (x: int_t t sec { v x < pow2 (size) })
+  (y: int_t t sec { v y < pow2 (size) })
+: Tot (z: int_t t sec { v z == (if v x <= v y then 1 else 0) })
+  (decreases (size))
+= if size = 0
+  then secret_bool true
+  else
+    let xh = highest_bit size x in
+    let xl = lowest_bits size x in
+    let yh = highest_bit size y in
+    let yl = lowest_bits size y in
+    (xh `one_bit_lt` yh) `logor_one_bit`
+    ((xh `one_bit_eq` yh) `logand_one_bit` secret_is_le (size - 1) xl yl)
